trunk/examples/programs/regression/bpl/TestQuantifierEliminationInequality03.bpl
@@ -9,6 +9,7 @@ var upper, lower, x, a,b,c: int;
 
 
 procedure proc() returns ()
+modifies a, b;
 {
   assume upper >= x;
   assume x >= lower;
@@ -22,7 +23,11 @@ procedure proc() returns ()
   while (*) {
     //prevent large block encoding
   }
+//   a := a+1;
+//   b := b+1;
   assert upper >= lower + 2;
+
+
 }
 
 
