trunk/examples/programs/regression/bpl/TestQuantifierEliminationInequality03_WithConstants.bpl
@@ -1,6 +1,6 @@
 //#Safe
 /*
- * Author: heizmann@informatik.uni-freiburg.de, musab@informatik.uni-freiburg.de
+ * Author: heizmann@informatik.uni-freiburg.de
  * Date: 2.11.2014
  * 
  */
@@ -9,20 +9,25 @@ var upper, lower, x, a,b,c: int;
 
 
 procedure proc() returns ()
+modifies a, b;
 {
-  assume upper >= x+2;
-  assume x+2 >= lower;
+  assume upper >= x;
+  assume x >= 0;
   assume a <= upper;
-  assume a >= lower;
+  assume a >= 0;
   assume b <= upper;
-  assume b >= lower;
-  assume x+2 != a;
-  assume x+2 != b;
+  assume b >= 0;
+  assume x != a;
+  assume x != b;
   assume a != b;
   while (*) {
     //prevent large block encoding
   }
-  assert upper >= lower + 2;
+//   a := a+1;
+//   b := b+1;
+  assert upper >= 2;
+
+
 }
 
 
